---
pagetitle: Factoring GCF
---

## Factoring

<details>
<summary>GCF Factoring</summary>
<p>

###### Rule

You can rewrite $(a \cdot b + a \cdot c)$ as $a \cdot (b + c)$ by dividing both terms of the expression by the `greatest common factor` in the following manner: 

\begin{align*}
    (a \cdot b + a \cdot c) &=& \\ 
    &= a\left(\frac{a \cdot b}{a} + \frac{a \cdot c}{a}\right) \\ 
    &= a(b + c)
\end{align*}

> Divide all terms of the expression by the `GCF` or `greatest common factor` and set the `GCF` out to the left of the parentheses.

###### Examples

1. Given: $(4a + 4b)$ factor the expression using the `GCF`.

    <details><summary>Show/Hide Solution</summary>
    <p>
        \begin{align*}
            (4a + 4b) &=& \\ 
            &= 4\left(\frac{4a}{4} + \frac{4b}{4}\right) \\ 
            &= 4(a + b)
        \end{align*}
    </p>
    </details>

2. Given: $(21x^4 + 33x^5)$ factor the expression using the `GCF`.

    <details><summary>Show/Hide Solution</summary>
    <p>
        \begin{align*}
            (21x^4 + 33x^5) &=& \\
            &= 3x^4\left(\frac{21x^4}{3x^4} + \frac{33x^5}{3x^4}\right) \\
            &= 3x^4\left(\frac{21}{3}x^{4-4} + \frac{33}{3}x^{5-4}\right) \\
            &= 3x^4(7x^0 + 11x^1) \textrm{   Recall }x^0=1\textrm{ and  }x^1=x \therefore \\
            &= 3x^4(7 + 11x)
        \end{align*}
    </p>
    </details>

3. Given: $(5x + 15x^2)$ factor the expression using the `GCF`.

    <details><summary>Show/Hide Solution</summary>
    <p>
