---
pagetitle: Polynomial Arithmetic
---

## Polynomial Arithmetic
<details><summary>Click here</summary>

### Definitions
<details><summary>Click here</summary>

#### Polynomial
* Poly means many.
* Nomial means term.
* $\therefore$ Polynomial means many terms.

#### Monomial
* Mono means one.
* Nomial means term.
* $\therefore$ Monomial means one term.

#### Binomial
* Bi means two.
* Nomial means term.
* $\therefore$ Binomial means two terms.

#### Trinomial
* Tri means three.
* Nomial means term.
* $\therefore$ Trinomial means three terms.

#### Polynomials with More Than Three Terms
* All polynomials with more than three terms is named according to the degree of the polynomial.
* The degree of a polynomial is equal to the highest degree of any term in the polynomial.
</details>


### Binomial Multiplication
Given $(a+b)(c+d)$ we distribute multiply each term in the first binomial to the second binomial, as follows:

\begin{split}
	(a+b)(c+d) &= a(c+d)+b(c+d) \\
		   &= ac + ad + bc + bd  \blacksquare
\end{split}

> Thus, we see that binomial multiplication is a means of transforming multiplication into addition. 

#### Examples

1. Given $(1+2)(3+4)$ use <code class="hl">binomial distribution</code> to multiply the binomials.

	Solution:
	
	\begin{align*}
		(1+2)(3+4) &= 1(3+4) + 2(3+4) \\
			   &= 1 \cdot 3 + 1 \cdot 4 + 2 \cdot 3 + 2 \cdot 4 \\
			   &= 3 + 4 + 6 + 8 \\
			   &= 21  \blacksquare
	\end{align*}

	This makes sense since $1+2=3$ and $3+4=7$ and $3 \times 7=21$.

2. Given $(2+1)(3+4)$ use binomial multiplication to `expand` the terms.

	Solutions:

	\begin{align*}
		(2+1)(3+4) &= 2(3+4) + 1(3+4) \\
			   &= 2 \cdot 3 + 2 \cdot 4 + 1 \cdot 3 + 1 \cdot 4 \\
			   &= 6 + 8 + 3 + 4 \\
			   &= 21 \blacksquare
	\end{align*}

	This example reminds us that `addition` is <code class="noun">commutative</code> which means the order of the `addends` *inside each parentheses* **does not matter**.
 
</details>
